dimsum/itree/rec.v
@@ -1,9 +1,6 @@
 From dimsum.core.itree Require Export upstream events.
-From dimsum.core Require Import universes module axioms.
+From dimsum.core Require Import universes module axioms itree_mod.
 From dimsum.examples Require Import rec.
-Import ITreeStdppNotations.
-
-Notation moduleE EV S := (choiceE +' visibleE EV +' stateE S).
 
 Local Open Scope Z_scope.
 
@@ -19,34 +16,34 @@ Definition rec_expr_itree (e : expr) : itree (callE expr val +' moduleE rec_even
   match e with
   | Val v => Ret v
   | BinOp e1 op e2 =>
-      v1 ← trigger (Recursion.Call e1);
-      v2 ← trigger (Recursion.Call e2);
+      v1 ← call e1;
+      v2 ← call e2;
       v ← eval_binop op v1 v2?;
       Ret v
   | Load e1 =>
-      v1 ← trigger (Recursion.Call e1);
+      v1 ← call e1;
       l ← val_to_loc v1?;
       h ← get_rec_heap;
       v ← (h.(h_heap) !! l)?;
       Ret v
   | Store e1 e2 =>
-      v1 ← trigger (Recursion.Call e1);
-      v2 ← trigger (Recursion.Call e2);
+      v1 ← call e1;
+      v2 ← call e2;
       l ← val_to_loc v1?;
       h ← get_rec_heap;
       assume (heap_alive h l);;
       set_rec_heap (heap_update h l v2);;
       Ret v2
   | If e1 e2 e3 =>
-      v1 ← trigger (Recursion.Call e1);
+      v1 ← call e1;
       b ← val_to_bool v1?;
       if b then
-        trigger (Recursion.Call e2)
+        call e2
       else
-        trigger (Recursion.Call e3)
+        call e3
   | LetE x e1 e2 =>
-      v1 ← trigger (Recursion.Call e1);
-      trigger (Recursion.Call (subst x v1 e2))
+      v1 ← call e1;
+      call (subst x v1 e2)
   | AllocA xs e =>
       assume (Forall (λ x, 0 < x) xs.*2);;
       h ← get_rec_heap;
@@ -54,7 +51,7 @@ Definition rec_expr_itree (e : expr) : itree (callE expr val +' moduleE rec_even
       h' ← demonic _;
       assert (heap_alloc_list xs.*2 ls h h');;
       set_rec_heap h';;
-      v ← trigger (Recursion.Call (subst_l xs.*1 (ValLoc <$> ls) e));
+      v ← call (subst_l xs.*1 (ValLoc <$> ls) e);
       he ← get_rec_heap;
       he' ← angelic _;
       assume (heap_free_list (zip ls xs.*2) he he');;
@@ -65,11 +62,11 @@ Definition rec_expr_itree (e : expr) : itree (callE expr val +' moduleE rec_even
       fns ← get_rec_fns;
       if fns !! f is Some fn then
         assume (length vs = length fn.(fd_args));;
-        trigger (Recursion.Call (AllocA fn.(fd_vars) (subst_l fn.(fd_args) vs fn.(fd_body))))
+        call (AllocA fn.(fd_vars) (subst_l fn.(fd_args) vs fn.(fd_body)))
       else
         h ← get_rec_heap;
         visible (Outgoing, ERCall f vs h);;
-        trigger (Recursion.Call (Waiting true))
+        call (Waiting true)
   | Waiting b =>
       c ← demonic bool;
       if c then
@@ -80,10 +77,10 @@ Definition rec_expr_itree (e : expr) : itree (callE expr val +' moduleE rec_even
         fn ← (fns !! f)!;
         set_rec_heap h;;
         visible (Incoming, ERCall f vs h);;
-        v ← trigger (Recursion.Call (Call f (Val <$> vs)));
+        v ← call (Call f (Val <$> vs));
         h ← get_rec_heap;
         visible (Outgoing, ERReturn v h);;
-        trigger (Recursion.Call (Waiting b))
+        call (Waiting b)
       else
         assert (b = true);;
         v ← demonic _;
@@ -96,4 +93,107 @@ Definition rec_expr_itree (e : expr) : itree (callE expr val +' moduleE rec_even
   end%itree.
 
 Definition rec_itree : itree (moduleE rec_event rec_state) void :=
-  ITree.bind (rec rec_expr_itree (Waiting false)) (λ _, NB).
+  ITree.bind (rec' rec_expr_itree (Waiting false)) (λ _, NB).
+
+Local Ltac go :=
+  clear_itree.
+Local Ltac go_s :=
+  tstep_s; go.
+Local Ltac go_i :=
+  tstep_i; go.
+
+Lemma itree_tstep_bind_tau {E R} A h (x : itree _ A) cont:
+  ITreeTStep (E:=E) (R:=R) cont (ITree.bind (Tau x) h) (Tau (ITree.bind x h)).
+Proof. constructor. by rewrite unfold_bind. Qed.
+Global Hint Resolve itree_tstep_bind_tau : typeclass_instances.
+
+Lemma itree_tstep_interp_ret {E} {R A B S} f x cont (h : S → _):
+  ITreeTStep (E:=E) (R:=R) cont (ITree.bind (interp (recursive' (A:=A) (B:=B) f) (Ret x)) h) (ITree.bind (Ret x) h).
+Proof. constructor. by rewrite interp_ret. Qed.
+Global Hint Resolve itree_tstep_interp_ret : typeclass_instances.
+
+Lemma itree_tstep_interp_bind {E} {R A B S} f g1 (g2 : B → _) cont (h : S → _):
+  ITreeTStep (E:=E) (R:=R) cont
+    (ITree.bind (interp (recursive' (A:=A) (B:=B) f) (ITree.bind g1 g2)) h)
+    (ITree.bind (interp (recursive' f) g1) (λ x,
+         ITree.bind (interp (recursive' f) (g2 x)) h)).
+Proof. constructor. by rewrite interp_bind bind_bind. Qed.
+Global Hint Resolve itree_tstep_interp_bind : typeclass_instances.
+
+Lemma itree_tstep_interp_rec'_call {E} {R A B} f x (h : B → _):
+  ITreeTStep (E:=E) (R:=R) false
+    (ITree.bind (interp (recursive' (A:=A) (B:=B) f) (call x)) h)
+    (ITree.bind (Tau (rec' f x)) h).
+Proof.
+  constructor. rewrite interp_recursive'_call_eq.
+  do 3 f_equiv. setoid_rewrite tau_euttge. by rewrite bind_ret_r.
+Qed.
+Global Hint Resolve itree_tstep_interp_rec'_call : typeclass_instances.
+
+Class ITreeToTranslate {E1 E2 R} (i : itree E1 R) (H : E2 -< E1) (o : itree E2 R) := {
+    itree_to_translate : i ≅ translate (@resum _ _ _ _ H) o
+}.
+Global Hint Mode ITreeToTranslate + + + ! + - : typeclass_instances.
+
+Lemma itree_tstep_interp_rec'_inr {E} {R A B} f (g : itree (callE A B +' E) _)
+  (g' : itree E _) (h : B → _) cont :
+  ITreeToTranslate g _ g' →
+  ITreeTStep (E:=E) (R:=R) cont
+    (ITree.bind (interp (recursive' (A:=A) (B:=B) f) g) h)
+    (ITree.bind g' h).
+Proof.
+  move => [Heq]. constructor.
+  by rewrite Heq /= interp_translate /recursive' interp_trigger_h_ge.
+Qed.
+Global Hint Resolve itree_tstep_interp_rec'_inr : typeclass_instances.
+
+Global Instance ITreeToTranslate_assume_option E1 E2 R (o : option R) {HE1 : choiceE -< E1} (Hin : E1 -< E2) {HE2 : choiceE -< E2} :
+  (∀ T, TCEq (HE2 T) (cat (@resum _ _ _ _ HE1) (@resum _ _ _ _ Hin) T)) →
+  ITreeToTranslate (assume_option o) Hin (assume_option o).
+Proof.
+  move => /(_ void)/TCEq_eq Heq.
+  constructor. destruct o => //=.
+  - by rewrite translate_ret.
+  - rewrite /UB translate_bind /angelic translate_trigger_eq.
+    f_equiv; [|done]. by rewrite /subevent/resum/= Heq.
+Qed.
+
+
+Lemma itree_tstep_rec' {E} {R A B} f x  (h : B → _):
+  ITreeTStep (E:=E) (R:=R) false (ITree.bind (rec' (A:=A) (B:=B) f x) h) (ITree.bind (interp (recursive' f) (f x)) h).
+Proof. constructor. by rewrite rec'_as_interp_eq. Qed.
+Global Hint Resolve itree_tstep_rec' : typeclass_instances.
+
+
+Lemma rec_itree_refines_rec fns :
+  trefines (itree_mod rec_itree (rec_init fns)) (rec_mod fns).
+Proof.
+  apply: tsim_implies_trefines => n0 /=.
+  rewrite /rec_itree.
+  unshelve eapply tsim_remember. { simpl. exact (λ n '(t, Rec _ hi fnsi) '(Rec es hs fnss),
+    ∃ K e k,
+    t ⊒ ↓ᵢ (ITree.bind (rec' rec_expr_itree e) k) ∧
+    RecExprFill es K e ∧ hi = hs ∧ fnsi = fns ∧ fnss = fns ∧
+    ∀ v t' ei h', t' ⊒ ↓ᵢ (k v) → (t', Rec ei h' fns) ⪯{itree_trans rec_event rec_state, rec_trans, n, false} Rec (expr_fill K (Val v)) h' fns). }
+  { exists []. split!; [done|apply _|]. move => ?????/=. by go_i. } {
+    move => ?? [?[???]] [???] ? /= ?. destruct!. split!; [done..|]. move => *. apply: tsim_mono; naive_solver. }
+  move => n /= ? Hloop [?[???]] [???] [? [e ?]]. destruct!/=. go_i.
+  revert select (RecExprFill _ _ _) => -[?].
+  destruct e; simplify_eq/=.
+  - by tstep_s.
+  - go_i. by apply H5.
+  - go_i. go_i.
+    apply Hloop; [done|]. split!; [done|apply _|].
+    move => /= *.
+    go_i. go_i.
+    apply Hloop; [done|]. split!; [done|apply _|].
+    move => /= *.
+    go_s => ??.
+    go_i. split!. go.
+    go_i. by apply H5.
+  - go_i. go_i.
+    apply Hloop; [done|]. split!; [done|apply _|].
+    move => /= *.
+    go_s => *. simplify_eq/=.
+    go_i.
+Abort.
