dimsum/itree/upstream.v
@@ -29,3 +29,209 @@ Definition Tau_maybe {E R} (b : bool) (t : itree E R) :=
   if b then Tau t else t.
 Notation "'Tau?' b t" := (Tau_maybe b t)
   (at level 20, b at level 9, t at level 20, right associativity, format "'Tau?' b  t").
+
+Require Import Paco.paco.
+
+From Coq Require Import
+     Program.Tactics
+     Setoid
+     Morphisms.
+
+From ITree Require Import
+     Basics.Tacs
+     Basics.Category
+     Basics.Basics
+     Basics.Function
+     Core.ITreeDefinition
+     Core.KTree
+     Eq.Eqit
+     Eq.UpToTaus
+     Eq.Paco2
+     Indexed.Sum
+     Indexed.Function
+     Indexed.Relation
+     Interp.Handler
+     Interp.Interp
+     Interp.InterpFacts
+     Interp.Recursion.
+
+Global Instance eqit_false_true_rewrite {R E} r : RewriteRelation (@eqit E R R r false true) := { }.
+Global Instance eqit_true_false_rewrite {R E} r : RewriteRelation (@eqit E R R r true false) := { }.
+
+Lemma interp_trigger_eq {E F : Type -> Type} {R : Type}
+      (f : E ~> (itree F))
+      (e : E R) :
+  interp f (ITree.trigger e) ≅ ITree.bind (f _ e) (fun x => Tau (Ret x)).
+Proof.
+  unfold ITree.trigger. rewrite interp_vis.
+  setoid_rewrite interp_ret.
+  reflexivity.
+Qed.
+
+(* We cannot have ≅ here because interp inserts a Tau after every
+visible event in t. *)
+Lemma interp_trigger_h_ge {E R} (t : itree E R) :
+  interp ITree.trigger t ≳ t.
+Proof. apply interp_id_h. Qed.
+
+Lemma translate_trigger_eq {E F G} `{E -< F} :
+  forall X (e: E X) (h: F ~> G),
+    translate h (trigger e) ≅ trigger (h _ (subevent X e)).
+Proof.
+  intros; unfold trigger; rewrite translate_vis; setoid_rewrite translate_ret; reflexivity.
+Qed.
+
+#[global]
+Instance euttge_cong_eq {E R1 R2 RR}:
+  Proper (eq_itree eq ==> eq_itree eq ==> iff)
+    (@eqit E R1 R2 RR true false).
+Proof. split; ginit; intros; [rewrite <-H, <-H0|rewrite H, H0]; eauto with paco. Qed.
+
+Definition interp_mrec' {D E : Type -> Type}
+           (ctx : D ~> itree (D +' E)) : itree (D +' E) ~> itree E :=
+  fun R =>
+    ITree.iter (fun t : itree (D +' E) R =>
+      match observe t with
+      | RetF r => Ret (inr r)
+      | TauF t => Ret (inl t)
+      | VisF (inl1 d) k => Ret (inl (ITree.bind (ctx _ d) (fun x => Tau (k x))))
+      | VisF (inr1 e) k => Vis e (fun x => Ret (inl (k x)))
+      end).
+
+Arguments interp_mrec' {D E} & ctx [T].
+
+Definition mrec' {D E : Type -> Type}
+           (ctx : D ~> itree (D +' E)) : D ~> itree E :=
+  fun R d => interp_mrec' ctx (ctx _ d).
+
+Arguments mrec' {D E} & ctx [T].
+
+Definition rec' {E : Type -> Type} {A B : Type}
+           (body : A -> itree (callE A B +' E) B) :
+  A -> itree E B :=
+  fun a => mrec' (calling' body) (Call a).
+
+Arguments rec' {E A B} &.
+
+Section Facts.
+Context {D E : Type -> Type} (ctx : D ~> itree (D +' E)).
+
+Definition _interp_mrec' {R : Type} (ot : itreeF (D +' E) R _) : itree E R :=
+  match ot with
+  | RetF r => Ret r
+  | TauF t => Tau (interp_mrec' ctx t)
+  | VisF e k =>
+    match e with
+    | inl1 d => Tau (interp_mrec' ctx ((ITree.bind (ctx _ d) (fun x => Tau (k x)))))
+    | inr1 e => Vis e (fun x => Tau (interp_mrec' ctx (k x)))
+    end
+  end.
+
+
+Lemma unfold_interp_mrec' R (t : itree (D +' E) R) :
+  interp_mrec' ctx t ≅ _interp_mrec' (observe t).
+Proof.
+  unfold interp_mrec'.
+  rewrite unfold_iter.
+  destruct observe; cbn.
+  - rewrite bind_ret_l; reflexivity.
+  - rewrite bind_ret_l. pstep; constructor. intros. left. apply reflexivity.
+  - destruct e; cbn.
+    + rewrite bind_ret_l; reflexivity.
+    + rewrite bind_vis.
+      pstep; constructor. intros. left.
+      rewrite bind_ret_l.
+      apply reflexivity.
+Qed.
+
+Definition mrecursive' (f : D ~> itree (D +' E))
+  : (D +' E) ~> itree E := fun _ m =>
+  match m with
+  | inl1 m => Tau (mrec' f m)
+  | inr1 m => ITree.trigger m
+  end.
+
+Global Instance eq_itree_mrec' {R} :
+  Proper (eq_itree eq ==> eq_itree eq) (@interp_mrec' _ _ ctx R).
+Proof.
+  ginit. pcofix CIH. intros.
+  rewrite !unfold_interp_mrec'.
+  punfold H0. inv H0; try discriminate; pclearbot; simpobs; [| |destruct e]; gstep.
+  - apply reflexivity.
+  - econstructor. eauto with paco.
+  - econstructor. gbase. eapply CIH. apply eqit_bind; auto; [reflexivity|].
+    intros ?. pstep; constructor. left. eauto.
+  - econstructor. gstep; constructor. auto with paco itree.
+Qed.
+
+
+Theorem interp_mrec_bind' {U T} (t : itree _ U) (k : U -> itree _ T) :
+  interp_mrec' ctx (ITree.bind t k) ≅
+  ITree.bind (interp_mrec' ctx t) (fun x => interp_mrec' ctx (k x)).
+Proof.
+  revert t k; ginit. pcofix CIH; intros.
+  rewrite (unfold_interp_mrec' _ t).
+  rewrite (unfold_bind t).
+  destruct (observe t); cbn;
+    [| |destruct e];
+    autorewrite with itree.
+  1: apply reflexivity.
+  all: rewrite unfold_interp_mrec'; ITree.fold_subst.
+  all: try (gstep; econstructor; eauto with paco).
+  - setoid_rewrite <-bind_tau. rewrite <-bind_bind. eauto with paco.
+  - intros. red. rewrite bind_tau. gstep; constructor; auto with paco.
+Qed.
+
+Theorem interp_mrec'_as_interp_eq {T} (c : itree _ T) :
+  interp_mrec' ctx c ≅ interp (mrecursive' ctx) c.
+Proof.
+  revert_until T. ginit. pcofix CIH. intros.
+  rewrite unfold_interp_mrec', unfold_interp.
+  destruct (observe c); [| |destruct e]; simpl; eauto with paco.
+  - gstep; repeat econstructor; eauto.
+  - gstep; constructor; eauto with paco.
+  - rewrite bind_tau. rewrite interp_mrec_bind'. unfold mrec'.
+    gstep; constructor.
+    guclo eqit_clo_bind; econstructor; [reflexivity|].
+    intros ? _ []. rewrite unfold_interp_mrec'. cbn.
+    gstep; constructor. eauto with paco.
+  - unfold ITree.trigger, case_; simpl. rewrite bind_vis.
+    gstep. constructor.
+    intros; red.
+    rewrite bind_ret_l.
+    gstep. constructor.
+    auto with paco.
+Qed.
+
+Theorem mrec'_as_interp_eq {T} (d : D T) :
+  mrec' ctx d ≅ interp (mrecursive' ctx) (ctx _ d).
+Proof.
+  apply interp_mrec'_as_interp_eq.
+Qed.
+
+End Facts.
+
+Local Opaque interp_mrec'.
+
+(** [rec' body] is equivalent to [interp (recursive' body)],
+    where [recursive'] is defined as follows. *)
+Definition recursive' {E A B} (f : A -> itree (callE A B +' E) B) : (callE A B +' E) ~> itree E :=
+  case_ (calling' (fun a => Tau (rec' f a))) ITree.trigger.
+
+Lemma rec'_as_interp_eq {E A B} (f : A -> itree (callE A B +' E) B) (x : A) :
+  rec' f x ≅ interp (recursive' f) (f x).
+Proof.
+  unfold rec'.
+  rewrite mrec'_as_interp_eq.
+  eapply eq_itree_interp.
+  - red. unfold case_; intros ? [[] | ]; reflexivity.
+  - reflexivity.
+Qed.
+
+Lemma interp_recursive'_call_eq {E A B} (f : A -> itree (callE A B +' E) B) (x:A) :
+   interp (recursive' f) (call x) ≅ Tau (ITree.bind (rec' f x) (fun x => Tau (Ret x))).
+Proof.
+  unfold recursive'. unfold call.
+  rewrite interp_trigger_eq. cbn.
+  rewrite bind_tau. reflexivity.
+Qed.
